user 7, session 173, part 37

diffs-w-failures/7/user-7-session-173.v
@@ -102,4 +102,37 @@ Fixpoint subst (x : id) (s t : ty) {measure size t : ty :=
   | TVar y => if beq_id x y then s else t
   | TEV y => t
   end.
-Show.
+Next Obligation.
+(simpl).
+Set Silent.
+Omega.omega.
+Qed.
+Next Obligation.
+(simpl).
+Omega.omega.
+Qed.
+Next Obligation.
+(simpl).
+Omega.omega.
+Qed.
+Next Obligation.
+(simpl).
+Omega.omega.
+Qed.
+Next Obligation.
+(simpl).
+(rewrite rename__size).
+Omega.omega.
+Unset Silent.
+Qed.
+Notation "'[' x ':=' s ']' t" := (subst x s t) (at level 30) : btjt_scope.
+Set Silent.
+Lemma triv : forall (X : id) (s : ty) (t1 t2 : ty), [X := s] TPair t1 t2 = TPair ([X := s] t1) ([X := t2] t2).
+Proof.
+Unset Silent.
+(intros X s t1 t2).
+(unfold subst).
+(unfold subst_func).
+(unfold Fix_sub).
+(simpl).
+reflexivity.
